Abstract/Abstract.thy
@@ -15,9 +15,9 @@ where
   "get_nonce \<equiv> unknown"
 
 definition
-  read_passphrase :: "(string TPM.STORED_DATA) s_monad"
+  read_passphrase :: "nat \<Rightarrow> (string TPM.STORED_DATA) E_monad"
 where
-  "read_passphrase \<equiv> TPM_NV_ReadValue 4 0 None <catch> (\<lambda>e. exit_r)"
+  "read_passphrase i \<equiv> TPM_NV_ReadValue i 0 None"
 
 definition
   A_proc :: "(astate, astate) data_type"
@@ -25,7 +25,7 @@ where
   "A_proc \<equiv> \<lparr>
     Init = \<lambda>s. {s},
     Fin = id,
-    Run = lift_nd read_passphrase
+    Run = lift_nd (read_passphrase 4)
   \<rparr>"
 
 end
