Proofs/StateRelation.thy
@@ -4,7 +4,7 @@ imports
   "../Abstract/Abstract"
 begin
 
-context sable_verified
+context sable_verified_pp
 begin
 
 definition
